theories/Proofs.v
@@ -1,11 +1,463 @@
 (** * Proofs: definition of free-variable tableaux proofs. *)
 
+(** In this file, we define the free-variable tableau method as an "expansion" method,
+    i.e., we define a [Tableau] as a proof tree, and a [TableauProof] is a [Sequence] of
+    [Tableau]x such that an [ExpansionRule] is applied between every [Tableau] of the
+    [Sequence]. We define what it means for a [TableauProof] to be closed, and show that,
+    list of formulas [Neg F :: Gamma], if this context has a tableau proof, then [Gamma |= F]. *)
+
 From Stdlib Require Import Classical.
 From Stdlib Require Import Lia.
 
 From Tableaux Require Import Semantics.
 From Tableaux Require Import Skolemization.
 From Tableaux Require Import Syntax.
+
+Notation "x \in l" := (List.In x l) (at level 30).
+
+(** ** Tableaux *)
+Section Tableaux.
+  Context `{set_nat : set nat} {pred func var : Atom} (sko : Skolemization_ pred func var).
+
+  Let Form := Form_ pred func var.
+
+  Inductive TableauTree : Type :=
+  | Leaf
+  | Node (T1 : TableauTree) (Gamma : list Form) (T2 : TableauTree) : TableauTree.
+
+  Inductive BranchingStep : Type := Left | Right.
+
+  #[global] Instance EqDec_BranchingStep : EqDec BranchingStep.
+  Proof using Type.
+    intros [] [].
+    - now left.
+    - now right.
+    - now right.
+    - now left.
+  Qed.
+
+  (** A [Branch] of a tableau is a succession of [BranchingStep]s. *)
+  Definition Branch := list BranchingStep.
+
+  (** A [Branch] [is_branch_of] a [TableauTree] whenever the list of branching steps describes
+      a path from the root of the [TableauTree] to a node without children. *)
+  Inductive is_branch_of : Branch -> TableauTree -> Prop :=
+  | is_branch_of_nil : forall (Gamma : list Form), is_branch_of [] (Node Leaf Gamma Leaf)
+  | is_branch_of_left :
+    forall (T1 T2 : TableauTree) (Gamma : list Form) (B : Branch),
+      is_branch_of B T1 -> is_branch_of (Left :: B) (Node T1 Gamma T2)
+  | is_branch_of_right :
+    forall (T1 T2 : TableauTree) (Gamma : list Form) (B : Branch),
+      is_branch_of B T2 -> is_branch_of (Right :: B) (Node T1 Gamma T2).
+
+  (** A [Form]ula [F] [is_on_branch] [B] if it appears in any one of the nodes along [B]. *)
+  Inductive is_on_branch (F : Form) : Branch -> TableauTree -> Prop :=
+  | is_on_branch_node :
+    forall (T1 T2 : TableauTree) (Gamma : list Form) (B : Branch),
+      F \in Gamma -> is_on_branch F B (Node T1 Gamma T2)
+  | is_on_branch_left :
+    forall (T1 T2 : TableauTree) (Gamma : list Form) (B : Branch),
+      is_on_branch F B T1 -> is_on_branch F (Left :: B) (Node T1 Gamma T2)
+  | is_on_branch_right :
+    forall (T1 T2 : TableauTree) (Gamma : list Form) (B : Branch),
+      is_on_branch F B T2 -> is_on_branch F (Right :: B) (Node T1 Gamma T2).
+
+  Definition mkOptionalNode (Gamma : option (list Form)) :=
+    match Gamma with
+    | Some Gamma => Node Leaf Gamma Leaf
+    | None => Leaf
+    end.
+
+  Fixpoint expand_tableau_branch__aux (left_forms right_forms : option (list Form))
+    (B : Branch) (T : TableauTree) : option TableauTree :=
+    match B with
+    | [] =>
+        match T with
+        | Node Leaf Gamma Leaf => Some (Node (mkOptionalNode left_forms) Gamma (mkOptionalNode right_forms))
+        | _ => None
+        end
+    | b :: B =>
+        match T with
+        | Leaf => None
+        | Node T1 Gamma T2 =>
+            match b with
+            | Left => expand_tableau_branch__aux left_forms right_forms B T1 >>=
+                       (fun T1 => Some (Node T1 Gamma T2))
+            | Right => expand_tableau_branch__aux left_forms right_forms B T2 >>=
+                        (fun T2 => Some (Node T1 Gamma T2))
+            end
+        end
+    end.
+
+  (** The [context] of a branch is the list of all the formulas of a branch. *)
+  Fixpoint get_context (B : Branch) (T : TableauTree) : list Form :=
+    match T with
+    | Leaf => []
+    | Node T1 Gamma T2 => Gamma ++ (match B with
+                           | [] => []
+                           | Left :: B => get_context B T1
+                           | Right :: B => get_context B T2
+                           end)%list
+    end.
+
+  (** Actually, a [Tableau_] also keeps in memory the Skolem symbols introduced. *)
+  Record Tableau_ :=
+    { tree :> TableauTree
+    ; symbols : sko_record sko }.
+
+  Definition expand_tableau_branch (left_forms right_forms : option (list Form))
+    (B : Branch) (T : Tableau_) : option Tableau_ :=
+    expand_tableau_branch__aux left_forms right_forms B T >>=
+      (fun tree => Some {| tree := tree; symbols := symbols T |}).
+
+  (** A [Sequence] is a list of tableaux. *)
+  Definition Sequence := list Tableau_.
+
+  (** A [Tableau_] is said closed under a substitution if every branch has a contradiction. *)
+  Definition is_tableau_closed (T : Tableau_) (sigma : Substitution var (Term_ func var)) : Prop :=
+    forall (B : Branch),
+      is_branch_of B T ->
+      Bot \in get_context B T \/
+        (exists (F G : Form),
+            F \in get_context B T /\ G \in get_context B T /\
+              F@[sigma] = Neg G@[sigma]).
+
+  (** A [Branch] of a [Tableau_] is satisfied if its context is satisfied. *)
+  Definition exists_satisfied_branch (M : Model pred func) (mu : env M var) (T : Tableau_) : Prop :=
+    exists (B : Branch),
+      is_branch_of B T /\ [[ M # [] # mu '|= ls_to_form (get_context B T) ]].
+
+  (** A [Tableau_] is said satisfiable if there exists a model such that for every free-variable
+      environment, there is a branch that is satisfied. *)
+  Definition is_tableau_satisfiable (T : Tableau_) :=
+    exists (M : Model pred func), forall (mu : env M var), exists_satisfied_branch M mu T.
+
+  Definition mkTableau (Gamma : list Form) : Tableau_ :=
+    {| tree := Node Leaf Gamma Leaf
+    ;  symbols := empty_record |}.
+
+  Definition mkLeaf : Tableau_ := {| tree := Leaf; symbols := empty_record |}.
+
+  Lemma is_branch_of_extend_left :
+    forall (T T' : TableauTree) (B : Branch) (l : list Form) (l' : option (list Form)),
+      is_branch_of B T -> expand_tableau_branch__aux (Some l) l' B T = Some T' ->
+      is_branch_of (B ++ [Left])%list T'.
+  Proof using Type.
+    intros ????? hbranchof e. generalize dependent T'; induction hbranchof; intros T' e; cbn in *.
+    - injection e => <-; cbn. apply is_branch_of_left; constructor.
+    - destruct (expand_tableau_branch__aux (Some l) l' B T1) eqn:eT'.
+      + injection e => <-; cbn. apply is_branch_of_left; auto.
+      + inversion e.
+    - destruct (expand_tableau_branch__aux (Some l) l' B T2) eqn:eT'.
+      + injection e => <-; cbn. apply is_branch_of_right; auto.
+      + inversion e.
+  Qed.
+
+  Lemma is_branch_of_extend_right :
+    forall (T T' : TableauTree) (B : Branch) (l : option (list Form)) (l' : list Form),
+      is_branch_of B T -> expand_tableau_branch__aux l (Some l') B T = Some T' ->
+      is_branch_of (B ++ [Right])%list T'.
+  Proof using Type.
+    intros ????? hbranchof e. generalize dependent T'; induction hbranchof; intros T' e; cbn in *.
+    - injection e => <-; cbn. apply is_branch_of_right; constructor.
+    - destruct (expand_tableau_branch__aux l (Some l') B T1) eqn:eT'.
+      + injection e => <-; cbn. apply is_branch_of_left; auto.
+      + inversion e.
+    - destruct (expand_tableau_branch__aux l (Some l') B T2) eqn:eT'.
+      + injection e => <-; cbn. apply is_branch_of_right; auto.
+      + inversion e.
+  Qed.
+
+  Lemma is_branch_of_extend_None :
+    forall (T T' : TableauTree) (B : Branch),
+      is_branch_of B T -> expand_tableau_branch__aux None None B T = Some T' ->
+      is_branch_of B T'.
+  Proof using Type.
+    intros ??? hbranchof e. generalize dependent T'; induction hbranchof; intros T' e; cbn in *.
+    - injection e => <-; cbn. apply is_branch_of_nil.
+    - destruct (expand_tableau_branch__aux None None B T1) eqn:eT'.
+      + injection e => <-; cbn. apply is_branch_of_left; auto.
+      + inversion e.
+    - destruct (expand_tableau_branch__aux None None B T2) eqn:eT'.
+      + injection e => <-; cbn. apply is_branch_of_right; auto.
+      + inversion e.
+  Qed.
+
+  Lemma get_context_extend_left :
+    forall (T T' : TableauTree) (B : Branch) (Gamma l : list Form) (l' : option (list Form)),
+      is_branch_of B T -> expand_tableau_branch__aux (Some l) l' B T = Some T' ->
+      get_context B T = Gamma -> get_context (B ++ [Left])%list T' = (Gamma ++ l)%list.
+  Proof using Type.
+    intro T. induction T; intros ????? hbranchof e eT; destruct B.
+    - inversion e.
+    - inversion e.
+    - inversion hbranchof; subst. cbn in e.
+      injection e => <-; cbn. now rewrite !app_nil_r.
+    - destruct b; cbn.
+      + inversion hbranchof; subst.
+        cbn in e. destruct (expand_tableau_branch__aux (Some l) l' B T1) eqn:eT1.
+        * injection e => <-; cbn in *. erewrite IHT1; eauto.
+          rewrite app_assoc //.
+        * inversion e.
+      + inversion hbranchof; subst.
+        cbn in e. destruct (expand_tableau_branch__aux (Some l) l' B T2) eqn:eT2.
+        * injection e => <-; cbn in *. erewrite IHT2; eauto.
+          rewrite app_assoc //.
+        * inversion e.
+  Qed.
+
+  Lemma get_context_extend_right :
+    forall (T T' : TableauTree) (B : Branch) (Gamma l' : list Form) (l : option (list Form)),
+      is_branch_of B T -> expand_tableau_branch__aux l (Some l') B T = Some T' ->
+      get_context B T = Gamma -> get_context (B ++ [Right])%list T' = (Gamma ++ l')%list.
+  Proof using Type.
+    intro T. induction T; intros ????? hbranchof e eT; destruct B.
+    - inversion e.
+    - inversion e.
+    - inversion hbranchof; subst. cbn in e.
+      injection e => <-; cbn. now rewrite !app_nil_r.
+    - destruct b; cbn.
+      + inversion hbranchof; subst.
+        cbn in e. destruct (expand_tableau_branch__aux l (Some l') B T1) eqn:eT1.
+        * injection e => <-; cbn in *. erewrite IHT1; eauto.
+          rewrite app_assoc //.
+        * inversion e.
+      + inversion hbranchof; subst.
+        cbn in e. destruct (expand_tableau_branch__aux l (Some l') B T2) eqn:eT2.
+        * injection e => <-; cbn in *. erewrite IHT2; eauto.
+          rewrite app_assoc //.
+        * inversion e.
+  Qed.
+
+  (** An optional list of formulas is satisfied either if it is none or if the list is
+      satisfied. *)
+  Definition is_optional_satisfied
+    (M : Model pred func) (mu : env M var) (l : option (list Form)) :=
+    match l with
+    | None => False
+    | Some l => [[ M # [] # mu '|= ls_to_form l ]]
+    end.
+
+  (** If a satisfiable tableau is extended with lists of formulas of which one of them is also
+      satisfied by the same model, then the extended tableau is also satisfiable. *)
+  Lemma is_satisfiable_extend :
+    forall (M : Model pred func) (mu : env M var) (T T' : Tableau_) (B : Branch)
+      (l l' : option (list Form)),
+      is_branch_of B T -> expand_tableau_branch l l' B T = Some T' ->
+      is_optional_satisfied M mu l \/ is_optional_satisfied M mu l' ->
+      exists_satisfied_branch M mu T -> exists_satisfied_branch M mu T'.
+  Proof.
+    intros ?? [T symbs] [T' symbs'] ??? hbranchof e [hsatl | hsatl'] (B & hbranchB & hsatB);
+      cbn in e.
+
+    (* Case: the extension with the formulas on the left is satisfied. *)
+    - destruct (B == B0).
+
+      (* Case: the branch that was satisfied is, in fact, [B0]. *)
+      + destruct l.
+        * exists (List.app B [Left]); split; cbn.
+          -- rewrite e0. destruct (expand_tableau_branch__aux (Some l) l' B0 T) eqn:eT.
+             ++ eapply is_branch_of_extend_left; eauto.
+                injection e => ? <-; eauto.
+             ++ inversion e.
+          -- rewrite -e0 in e. destruct (expand_tableau_branch__aux (Some l) l' B T) eqn:eT.
+             ++ injection e => _ eT'. rewrite eT' in eT. erewrite get_context_extend_left; eauto.
+                cbn. unfold interpret; rewrite (ls_to_form_app (get_context B T) l M [] mu).
+                cbn. intros [hnB | hl]; auto.
+             ++ inversion e.
+        * now cbn in hsatl.
+
+      (* Case: the branch that was satisfied is not [B0]. *)
+      + exists B; split; admit.
+
+    (* Case: the extension with the formulas on the right is satisfied. *)
+    - destruct (B == B0).
+
+      (* Case: the branch that was satisfied is, in fact, [B0]. *)
+      + destruct l'.
+        * exists (B ++ [Right])%list; split; cbn.
+          -- rewrite e0. destruct (expand_tableau_branch__aux l (Some l0) B0 T) eqn:eT.
+             ++ eapply is_branch_of_extend_right; eauto.
+                injection e => ? <-; eauto.
+             ++ inversion e.
+          -- rewrite -e0 in e. destruct (expand_tableau_branch__aux l (Some l0) B T) eqn:eT.
+             ++ injection e => _ eT'; rewrite eT' in eT.
+                erewrite get_context_extend_right; eauto.
+                cbn; unfold interpret. rewrite (ls_to_form_app (get_context B T) l0 M [] mu).
+                cbn. intros [hnB | hl0]; auto.
+             ++ inversion e.
+
+        * inversion hsatl'.
+
+      (* Case: the branch that was satisfied is not [B0]. *)
+      + exists B; split; admit.
+  Admitted.
+End Tableaux.
+
+Arguments tree {_ _ _ _}.
+Arguments symbols {_ _ _ _}.
+Arguments is_tableau_closed {_ _ _ _ _} _ _.
+Arguments exists_satisfied_branch {_ _ _ _} _ _ _.
+
+(** ** Expansion rules *)
+
+(** We denote [T |> T'] when a [Tableau] [T] can be expanded to a tableau [T']. *)
+Reserved Notation "T |> T'" (at level 30, right associativity).
+Section ExpansionRules.
+  Context `{set_nat : set nat} {pred func var : Atom} (sko : Skolemization_ pred func var).
+
+  Let Term := Term_ func var.
+  Let Form := Form_ pred func var.
+  Let Tableau := Tableau_ sko.
+
+  (** By convention, we expand a tableau on the left side for unary rules. *)
+  Inductive ExpansionStep : Tableau -> Tableau -> Prop :=
+  | expansion_NegNeg :
+    forall (T T' : Tableau) (B : Branch) (F : Form),
+      is_branch_of B T -> is_on_branch (Neg (Neg F)) B T ->
+      expand_tableau_branch sko (Some [F]) None B T = Some T' -> T |> T'
+
+  | expansion_NegOr :
+    forall (T T' : Tableau) (B : Branch) (F1 F2 : Form),
+      is_branch_of B T -> is_on_branch (Neg (Or F1 F2)) B T ->
+      expand_tableau_branch sko (Some [Neg F1 ; Neg F2]) None B T = Some T' -> T |> T'
+
+  | expansion_Or :
+    forall (T T' : Tableau) (B : Branch) (F1 F2 : Form),
+      is_branch_of B T -> is_on_branch (Or F1 F2) B T ->
+      expand_tableau_branch sko (Some [F1]) (Some [F2]) B T = Some T' -> T |> T'
+
+  | expansion_All :
+    forall (T T' : Tableau) (B : Branch) (F : Form) (x : var),
+      is_branch_of B T -> is_on_branch (All F) B T ->
+      expand_tableau_branch sko (Some [F{0 \to Free x}]) None B T = Some T' -> T |> T'
+
+  | expansion_NegAll :
+    forall (T T' : Tableau) (B : Branch) (F : Form) (t : Term)
+      (hsko : sko t (Neg (All F)) (symbols T) (get_context B T) = true),
+      is_branch_of B T -> is_on_branch (Neg (All F)) B T ->
+      expand_tableau_branch__aux (Some [F{0 \to t}]) None B T = Some (tree T') ->
+      symbols T' = add_symbol (symbol sko hsko) (Neg (All F)) (symbols T) ->
+      T |> T'
+  where "T |> T'" := (ExpansionStep T T').
+
+  (** A [Sequence] is an [ExpansionSequence] if every neighbouring [Tableau] are related
+      by an [ExpansionStep]. *)
+  Definition is_expansion_sequence (s : Sequence sko) : Prop :=
+    forall (i : nat) (T T' : Tableau),
+      s.(i) = Some T -> s.(S i) = Some T' -> T |> T'.
+
+  (** A sequence is a tableau proof if there it is an expansion sequence s.t. the first
+      tableau of the sequence has a simple node labelled by this list of formulas and the
+      last is closed under a substitution [sigma]. *)
+  Definition is_tableau_proof (Gamma : list Form) (sigma : Substitution var Term) (s : Sequence sko) : Prop :=
+    is_expansion_sequence s /\
+      hd_error s = Some (mkTableau sko Gamma) /\
+      is_tableau_closed (last s (mkLeaf sko)) sigma.
+
+  (** A list of formulas have a tableau if there exists a sequence that is a tableau proof *)
+  Definition hasTableau (Gamma : list Form) (sigma : Substitution var Term) : Prop :=
+    exists (s : Sequence sko), is_tableau_proof Gamma sigma s.
+End ExpansionRules.
+
+Arguments ExpansionStep {_ _ _ _} _ _.
+Notation "T |> T'" := (ExpansionStep T T').
+
+(** ** Soundness *)
+
+(** In this section, we show that this definition of tableaux is sound, i.e., if list of formulas
+    [Neg F :: Gamma] has a tableau, then [Gamma |= F]. *)
+Section Soundness.
+  Context `{set_nat : set nat} {pred func var : Atom} (sko : Skolemization_ pred func var).
+
+  Let Term := Term_ func var.
+  Let Form := Form_ pred func var.
+  Let Tableau := Tableau_ sko.
+
+  (** First, we show that the last tableau of a proof cannot be satisfiable. *)
+  Lemma hasTableau_not_satisfiable :
+    forall (M : Model pred func) (Gamma : list Form) (sigma : Substitution var Term) (s : Sequence sko),
+      is_tableau_proof sko Gamma sigma s ->
+      (forall (B : Branch),
+          is_branch_of B (last s (mkLeaf sko)) ->
+          ~ [[ M # [] # subst_to_env M sigma '|= ls_to_form (get_context B (last s (mkLeaf sko))) ]]).
+  Proof using Type.
+    intros ???? (_ & _ & hclosed) ? hB hsat.
+    destruct (hclosed B hB) as [ htrivial | [ F [ G  [ hinF [ hinG e ] ] ] ] ].
+    - have [] := in_form_list_interp htrivial hsat.
+    - have hF := in_form_list_interp hinF hsat.
+      have hG := in_form_list_interp hinG hsat.
+      rewrite -!subst_commutes_with_env_forms in hF, hG.
+      rewrite e in hF. now apply hF.
+  Qed.
+
+  (** Then, we show that every expansion sequence starting from a satisfiable tableau is
+      satisfiable. We even show that there exists one model that satisfies every element
+      of the sequence. *)
+
+  (** We start by showing that applying an [ExpansionStep] on a satisfiable tableau keeps
+      satisfiability. *)
+  Lemma subject_reduction :
+    forall (T T' : Tableau),
+      is_tableau_satisfiable sko T -> (T |> T') ->
+      is_tableau_satisfiable sko T'.
+  Proof using set_nat.
+    intros T T' hsat hred. destruct hred as
+      [ T T' B F hbranchof hcontains e |
+        T T' B F1 F2 hbranchof hcontains e |
+        T T' B F1 F2 hbranchof hcontains e |
+        T T' B F x hbranchof hcontains e |
+        T T' B F t hsko hbranchof hcontains etree esymbs ].
+
+    (* Case: [Neg (Neg F)] *)
+    - destruct hsat as (M & hsat). exists M; intro mu. specialize (hsat mu).
+      eapply is_satisfiable_extend; eauto. left.
+      intros [hnF | contra]; firstorder.
+      (* easy *)
+
+eapply is_satisfiable_is_satisfiable_add_in_branch; eauto.
+      apply equiv_imply. symmetry; apply neg_neg_equiv.
+
+    (* Case: [Neg (Or F1 F2)] *)
+    - eapply is_satisfiable_is_satisfiable_add_in_branch with
+        (F := Neg (Or F1 F2)) (T := add_in_branch T i (Neg F1)).
+      + eapply add_in_branch_get; eauto.
+      + eapply is_satisfiable_is_satisfiable_add_in_branch; eauto.
+        intros M sigma hinterp hF1. apply hinterp. now left.
+      + now apply branch_contains_add.
+      + intros M sigma hinterp hF2. apply hinterp. now right.
+
+    (* Case: [Or F1 F2] *)
+    - apply is_satisfiable_is_satisfiable_or; auto.
+
+    (* Case: [All F] *)
+    - eapply is_satisfiable_is_satisfiable_add_in_branch; eauto.
+      apply instantiate_imply_all. unfold isLocallyClosed; now cbn.
+
+    (* Case: [Neg (All F)] *)
+    - destruct hsat as (M & hsat0).
+      destruct (is_sko_sound H M) as (interp & hinterpsko & hinterp).
+      exists (ReplacementModel M interp); intro mu.
+      specialize (hsat0 mu). destruct hsat0 as (B0 & hin & hinterp0).
+      apply In_nth_error in hin; destruct hin as (k & ek).
+      destruct (i == k); subst.
+      + exists (B ,, Neg F {0 \to t}); split.
+        * unfold add_in_branch. rewrite H0.
+          eapply In_replace_nth; eauto.
+        * have eB0 : B = B0.
+          { unfold nth_branch_of in H0; rewrite H0 in ek; now injection ek. }
+          intros [hnF | hB].
+          -- apply hnF, hinterpsko.
+             eapply in_form_list_interp; eauto.
+             now rewrite eB0.
+          -- rewrite eB0 in hB; now apply hB, hinterp.
+      + exists B0; split.
+        * unfold add_in_branch. rewrite H0.
+          eapply In_replace_nth'; eauto.
+        * now apply hinterp.
+  Qed.
+
+End Soundness.
 
 (** ** Contexts *)
 
